src/Std/Data/DTreeMap/Lemmas.lean
@@ -1072,7 +1072,7 @@ theorem forIn_eq_forIn [Monad m] [LawfulMonad m]
 
 theorem forIn_eq_forIn_toList [Monad m] [LawfulMonad m]
     {f : (a : α) × β a → δ → m (ForInStep δ)} {init : δ} :
-    t.forIn (fun k v => f ⟨k, v⟩) init = ForIn.forIn t.toList init f :=
+    ForIn.forIn t init f = ForIn.forIn t.toList init f :=
   Impl.forIn_eq_forIn_toList (f := f)
 
 theorem foldlM_eq_foldlM_keys [Monad m] [LawfulMonad m] {f : δ → α → m δ} {init : δ} :
@@ -1093,12 +1093,12 @@ theorem foldr_eq_foldr_keys {f : α → δ → δ} {init : δ} :
   Impl.foldr_eq_foldr_keys
 
 theorem forM_eq_forM_keys [Monad m] [LawfulMonad m] {f : α → m PUnit} :
-    t.forM (fun a _ => f a) = t.keys.forM f :=
+    ForM.forM t (fun a => f a.1) = t.keys.forM f :=
   Impl.forM_eq_forM_keys
 
 theorem forIn_eq_forIn_keys [Monad m] [LawfulMonad m]
     {f : α → δ → m (ForInStep δ)} {init : δ} :
-    t.forIn (fun a _ d => f a d) init = ForIn.forIn t.keys init f :=
+    ForIn.forIn t init (fun a d => f a.1 d) = ForIn.forIn t.keys init f :=
   Impl.forIn_eq_forIn_keys
 
 namespace Const
@@ -1123,10 +1123,33 @@ theorem foldr_eq_foldr_toList {f : α → β → δ → δ} {init : δ} :
     t.foldr f init = (Const.toList t).foldr (fun a b => f a.1 a.2 b) init :=
   Impl.Const.foldr_eq_foldr_toList
 
+theorem forM_eq_forMUncurried [Monad m] [LawfulMonad m] {f : α → β → m PUnit} :
+    t.forM f = forMUncurried (fun a => f a.1 a.2) t := rfl
+
+theorem forMUncurried_eq_forM_toList [Monad m] [LawfulMonad m] {f : α × β → m PUnit} :
+    forMUncurried f t = (Const.toList t).forM f :=
+  Impl.Const.forM_eq_forM_toList
+
+/--
+Deprecated, use `forMUncurried_eq_forM_toList` together with `forM_eq_forMUncurried` instead.
+-/
+@[deprecated forMUncurried_eq_forM_toList (since := "2025-03-02")]
 theorem forM_eq_forM_toList [Monad m] [LawfulMonad m] {f : α → β → m PUnit} :
     t.forM f = (Const.toList t).forM (fun a => f a.1 a.2) :=
-  Impl.Const.forM_eq_forM_toList (f := f)
+  Impl.Const.forM_eq_forM_toList
 
+theorem forIn_eq_forInUncurried [Monad m] [LawfulMonad m]
+    {f : α → β → δ → m (ForInStep δ)} {init : δ} :
+    t.forIn f init = forInUncurried (fun a b => f a.1 a.2 b) init t := rfl
+
+theorem forInUncurried_eq_forIn_toList [Monad m] [LawfulMonad m]
+    {f : α × β → δ → m (ForInStep δ)} {init : δ} :
+    forInUncurried f init t = ForIn.forIn (Const.toList t) init f :=
+  Impl.Const.forIn_eq_forIn_toList
+
+/--
+Deprecated, use `forMUncurried_eq_forM_toList` together with `forM_eq_forMUncurried` instead.
+-/
 theorem forIn_eq_forIn_toList [Monad m] [LawfulMonad m]
     {f : α → β → δ → m (ForInStep δ)} {init : δ} :
     t.forIn f init = ForIn.forIn (Const.toList t) init (fun a b => f a.1 a.2 b) :=
